progress with initial_memory_from_data lemma

coq/LLVMGen/Data.v
@@ -335,8 +335,8 @@ Definition helix_initial_memory
        let '(data, y) := constMemBlock (MInt64asNT.to_nat o) data in
        let '(data, x) := constMemBlock (MInt64asNT.to_nat i) data in
        (* over-estimating id, as some globals may not alocate memory (e.g. scalars) *)
-       let X_nat : nat := length globals  in
-       let Y_nat : nat := S (length globals) in
+       let Y_nat : nat := length globals  in
+       let X_nat : nat := S (length globals) in
        let mem := memory_set mem Y_nat y in
        let mem := memory_set mem X_nat x in
        let σ := globals_σ ++ [(DSHPtrVal Y_nat o,false); (DSHPtrVal X_nat i,false)] in
